sme/Sme/ITree/Events/Empty.lean
@@ -1,0 +1,13 @@
+import Sme.ITree.Defs
+import Sme.ITree.Bisim
+import Sme.ITree.Monad
+import Sme.ITree.Combinators
+import Sme.ITree.MonadIter
+
+namespace Sme.ITree
+
+universe u v w
+
+inductive EmptyE : Type u → Type u
+
+end Sme.ITree
