sme/Sme/ITree/Events/Map.lean
@@ -1,0 +1,27 @@
+import Sme.ITree.Defs
+import Sme.ITree.Bisim
+import Sme.ITree.Monad
+import Sme.ITree.Combinators
+import Sme.ITree.MonadIter
+import Sme.ITree.Events.State
+import Std.Data.ExtHashMap.Basic
+
+namespace Sme.ITree
+
+universe u v w
+
+inductive MapE (K V : Type u) : Type u → Type u
+  | insert : K → V → MapE K V PUnit
+  | get : K → MapE K V (Option V)
+  | getD : K → V → MapE K V V
+  | erase : K → MapE K V PUnit
+
+def MapE.handle {K V : Type u} [BEq K] [EquivBEq K] [Hashable K] [LawfulHashable K]
+    : MapE K V ↝ (StateT (PLift (Std.ExtHashMap K V)) (ITree EmptyE) ∘ PLift) := fun
+  | _, .insert k v => fun hm => pure ⟨.up .unit, .up <| hm.down.insert k v⟩
+  | _, .get k => fun hm => pure ⟨.up <| hm.down.get? k, hm⟩
+  | _, .getD k v => fun hm => pure ⟨.up <| hm.down.getD k v, hm⟩
+  | _, .erase k => fun hm => pure ⟨.up .unit, .up <| hm.down.erase k⟩
+  /- | _, .put v => fun _ => pure ⟨.up .unit, .up v⟩ -/
+
+end Sme.ITree
