sme/Sme/ITree/Events/State.lean
@@ -2,6 +2,8 @@ import Sme.ITree.Defs
 import Sme.ITree.Bisim
 import Sme.ITree.Monad
 import Sme.ITree.Combinators
+import Sme.ITree.MonadIter
+import Sme.ITree.Events.Empty
 
 namespace Sme.ITree
 
@@ -11,16 +13,17 @@ inductive StateE (S : Type u) : Type u → Type u
   | get : StateE S S
   | put : S → StateE S PUnit
 
-def StateE.handle {E} {S} : StateE S ↝ StateT S (ITree E) := fun
+def StateE.handle {S : Type u} {E}
+    : StateE S ↝ (StateT (PLift S) (ITree E) ∘ PLift) := fun
   | _, .get => StateT.get
-  | _, .put v => StateT.set v
+  | _, .put v => fun _ => pure ⟨.up .unit, .up v⟩
 
-def StateE.interp {S E} : ITree (StateE S) ↝ StateT S (ITree E) :=
-  fun _ x s => ITree.iter (fun
-    | ⟨s, .ret v⟩ => .ret <| .inr ⟨v, s⟩
-    | ⟨s, .tau v⟩ => .ret <| .inl ⟨s, v.dest⟩
-    | ⟨s, .vis e v⟩ => ITree.map (fun ⟨a, s⟩ => .inl ⟨s, (v a).dest⟩) <| handle _ e s)
-    (Prod.mk s x.dest)
+instance {σ : Type u} {M : Type _ → Type _} [Iter M] [Functor M]
+    : Iter (StateT σ M) where
+  iter f a s := Iter.iter (fun ⟨a, s⟩ => (fun
+    | ⟨.inl x, y⟩ => .inl ⟨x, y⟩
+    | ⟨.inr x, y⟩ => .inr ⟨x, y⟩
+    ) <$> f a s) (Prod.mk a s)
 
 end Sme.ITree
 
