sme/Sme/ITree/Examples/Echo.lean
@@ -1,0 +1,14 @@
+import Sme.ITree.Interp
+import Sme.ITree.Events.State
+
+open Sme ITree
+
+def echo : ITree (StateE Nat) PEmpty :=
+  .iter (fun _ =>
+    .vis .get fun v =>
+    .vis (.put v) fun _ =>
+    .ret <| .inl .unit
+  ) Unit.unit
+
+#check interp StateE.handle _ echo
+
