sme/Sme/ITree/Examples/Imp.lean
@@ -1,0 +1,336 @@
+import Sme.ListMemT
+import Sme.HList
+import Sme.ITree.Interp
+import Sme.ITree.WBisim
+import Sme.ITree.Events.Map
+import Sme.ITree.Events.SubEvent
+
+open Sme ITree
+
+inductive Imp (N : Type) : Type
+  -- arith
+  | add (a b : Imp N)
+  | mul (a b : Imp N)
+  | sub (a b : Imp N)
+  | constN (n : Int)
+  -- variables
+  | var    (v : N)
+  | assign (k : N) (a : Imp N)
+  -- IO
+  | print (a : Imp N)
+  | seq (a b : Imp N)
+  -- control
+  | ite (c t f : Imp N)
+  | while (c b : Imp N)
+deriving DecidableEq
+
+inductive IOE : Type → Type
+  | print : Int → IOE Unit
+
+def sem {N} : Imp N → ITree (IOE ⊕, MapE N Int) Int
+  -- arith
+  | .add a b => do
+    let a ← sem a
+    let b ← sem b
+    return a + b
+  | .mul a b => do
+    let a ← sem a
+    let b ← sem b
+    return a * b
+  | .sub a b => do
+    let a ← sem a
+    let b ← sem b
+    return a - b
+  | .constN n => .ret n
+  -- var
+  | .var v => .trigger <| .inr <| .getD v 0
+  | .assign k v => do
+    let v ← sem v
+    let _ ← .trigger <| .inr <| .insert k v
+    return 0
+  -- effects
+  | .print v => do
+    let v ← sem v
+    let _ ← .trigger <| .inl <| .print v
+    return 0
+  | .seq a b => do
+    let _ ← sem a
+    sem b
+  -- control
+  | .while c b => .iter (fun _ => do
+      let c ← sem c
+      if c ≠ 0 then
+        let _ ← sem b
+        return .inl .unit
+      else
+        return .inr 0
+    ) Unit.unit
+  | .ite c t f => do
+    let c ← sem c
+    if c ≠ 0 then sem t
+    else          sem f
+
+def constProp {N} (inp : Imp N) : Imp N :=
+  flat <| pass inp
+where
+  flat : Int ⊕ _ → _
+    | .inl v => .constN v
+    | .inr v => v
+  pass : _ → Int ⊕ _
+    | .add a b =>
+      match pass a, pass b with
+      | .inl a, .inl b => .inl (a + b)
+      | .inr a, b => .inr <| .add a (flat b)
+      | .inl a, .inr b => .inr <| .add (.constN a) b
+    | .mul a b =>
+      match pass a, pass b with
+      | .inl a, .inl b => .inl (a * b)
+      | .inr a, b => .inr <| .mul a (flat b)
+      | .inl a, .inr b => .inr <| .mul (.constN a) b
+    | .sub a b =>
+      match pass a, pass b with
+      | .inl a, .inl b => .inl (a - b)
+      | .inr a, b => .inr <| .sub a (flat b)
+      | .inl a, .inr b => .inr <| .sub (.constN a) b
+    | .constN n => .inl n
+    | .print v => .inr <| .print <| flat (pass v)
+    | .var n => .inr <| .var n
+    | .assign n v => .inr <| .assign n <| flat (pass v)
+    | .seq a b =>
+      match pass a, pass b with
+      | .inl _, b => b
+      | .inr a, .inl b => .inr <| .seq a (.constN b)
+      | .inr a, .inr b => .inr <| .seq a b
+    | .ite c t f =>
+      match pass c, pass t, pass f with
+      | .inl 0, _, f => f
+      | .inl (.ofNat (_ + 1)), t, _ | .inl (.negSucc _), t, _ => t
+      | .inr c, t, f => .inr <| .ite c (flat t) (flat f)
+    | .while c b =>
+      match pass c, pass b with
+      | .inl 0, _ => .inl 0
+      | .inl (.ofNat (_ + 1)), b | .inl (.negSucc _), b =>
+        .inr <| .while (.constN 1) <| flat b
+      | .inr c, b => .inr <| .while c <| flat b
+
+open constProp in
+theorem pass_inl_eq_wbisim {N} {a : Imp N} {v}
+    (h : pass a = Sum.inl v)
+    : sem a ≈ .ret v :=
+  match a with
+  | .constN _ => by
+    obtain rfl := (Sum.inl.injEq _ _).mp h
+    rfl
+  | .add a b => by
+    dsimp [pass] at h
+    split at h
+    · rename_i a' b' h₁ h₂
+      obtain rfl := (Sum.inl.injEq _ _).mp h
+      have h₁ := pass_inl_eq_wbisim h₁
+      have h₂ := pass_inl_eq_wbisim h₂
+      change ((sem a).bind fun a ↦ (sem b).bind fun b ↦ pure (a + b)) ≈ pure _
+      trans (ITree.ret a').bind fun a ↦ (sem b).bind fun b ↦ pure (a + b)
+      · exact WBisim.bind_congr_arg h₁
+      rw [ret_bind]
+      trans ((ITree.ret b').bind fun b ↦ pure (a' + b))
+      · exact WBisim.bind_congr_arg h₂
+      rw [ret_bind]
+    · contradiction
+    · contradiction
+  | .sub a b => by
+    dsimp [pass] at h
+    split at h
+    · rename_i a' b' h₁ h₂
+      obtain rfl := (Sum.inl.injEq _ _).mp h
+      have h₁ := pass_inl_eq_wbisim h₁
+      have h₂ := pass_inl_eq_wbisim h₂
+      change ((sem a).bind fun a ↦ (sem b).bind fun b ↦ pure (a - b)) ≈ pure _
+      trans (ITree.ret a').bind fun a ↦ (sem b).bind fun b ↦ pure (a - b)
+      · exact WBisim.bind_congr_arg h₁
+      rw [ret_bind]
+      trans ((ITree.ret b').bind fun b ↦ pure (a' - b))
+      · exact WBisim.bind_congr_arg h₂
+      rw [ret_bind]
+    · contradiction
+    · contradiction
+  | .mul a b => by
+    dsimp [pass] at h
+    split at h
+    · rename_i a' b' h₁ h₂
+      obtain rfl := (Sum.inl.injEq _ _).mp h
+      have h₁ := pass_inl_eq_wbisim h₁
+      have h₂ := pass_inl_eq_wbisim h₂
+      change ((sem a).bind fun a ↦ (sem b).bind fun b ↦ pure (a * b)) ≈ pure _
+      trans (ITree.ret a').bind fun a ↦ (sem b).bind fun b ↦ pure (a * b)
+      · exact WBisim.bind_congr_arg h₁
+      rw [ret_bind]
+      trans ((ITree.ret b').bind fun b ↦ pure (a' * b))
+      · exact WBisim.bind_congr_arg h₂
+      rw [ret_bind]
+    · contradiction
+    · contradiction
+  | .var _
+  | .assign _ _
+  | .print _ => by
+    simp [pass] at h
+  | .seq a b => by
+    dsimp [pass] at h
+    split at h
+    · rename_i a' h'
+      have h₁ := pass_inl_eq_wbisim h'
+      have h₂ := pass_inl_eq_wbisim h
+      dsimp [sem, Bind.bind]
+      change ((sem a).bind fun _ ↦ sem b) ≈ ret v
+      trans ((ITree.ret a').bind fun _ ↦ sem b)
+      · exact WBisim.bind_congr_arg h₁
+      rw [ret_bind]
+      exact h₂
+    · contradiction
+    · contradiction
+  | .ite c t f => by
+    dsimp [pass, sem, Bind.bind] at h ⊢
+    split at h
+    · rename_i h'
+      have h₁ := pass_inl_eq_wbisim h'
+      have h₂ := pass_inl_eq_wbisim h
+      apply WBisim.trans (WBisim.bind_congr_arg h₁)
+      rw [ret_bind]
+      exact h₂
+    · rename_i h'
+      have h₁ := pass_inl_eq_wbisim h'
+      have h₂ := pass_inl_eq_wbisim h
+      apply WBisim.trans (WBisim.bind_congr_arg h₁)
+      rw [ret_bind]
+      exact h₂
+    · rename_i h'
+      have h₁ := pass_inl_eq_wbisim h'
+      have h₂ := pass_inl_eq_wbisim h
+      apply WBisim.trans (WBisim.bind_congr_arg h₁)
+      rw [ret_bind]
+      exact h₂
+    · contradiction
+  | .while c b => by
+    dsimp [pass, sem, Bind.bind] at h ⊢
+    split at h
+    · rename_i h₁
+      have h₁ := pass_inl_eq_wbisim h₁
+      obtain rfl := (Sum.inl.injEq _ _).mp h
+      rw [ITree.iter_eq, ITree.bind_assoc]
+      apply WBisim.trans (((WBisim.bind_congr_arg h₁)))
+      simp [pure]
+      rfl
+    · contradiction
+    · contradiction
+    · contradiction
+
+open constProp in
+mutual
+
+theorem pass_inr_eq_wbisim {N} {a : Imp N} {v}
+    (h : pass a = Sum.inr v)
+    : sem a ≈ sem v :=
+  match a with
+  | .constN _ => by
+    simp [pass] at h
+  | .mul a b | .sub a b | .add a b => by
+    dsimp [pass] at h
+    split at h
+    · contradiction
+    · obtain rfl := (Sum.inr.injEq _ _).mp h
+      rename_i a' h'
+      have h := pass_inr_eq_wbisim h'
+      dsimp [sem, Bind.bind]
+      apply WBisim.bind_congr h
+      intro a
+      dsimp
+      exact WBisim.bind_congr_arg constProp_safe
+    · obtain rfl := (Sum.inr.injEq _ _).mp h
+      rename_i h₁ h₂
+      apply WBisim.trans <| WBisim.bind_congr_arg <| pass_inl_eq_wbisim h₁
+      simp only [Bind.bind, ret_bind, sem]
+      exact WBisim.bind_congr_arg <| pass_inr_eq_wbisim h₂
+  | .var _ => by
+    obtain rfl := (Sum.inr.injEq _ _).mp h
+    rfl
+  | .assign _ _
+  | .print _ => by
+    obtain rfl := (Sum.inr.injEq _ _).mp h
+    dsimp [sem, Bind.bind]
+    apply WBisim.bind_congr_arg
+    exact constProp_safe
+  | .seq a b => by
+    dsimp [pass] at h
+    split at h
+    · rename_i h'
+      apply WBisim.trans <| WBisim.bind_congr_arg <| pass_inl_eq_wbisim h'
+      simp only [ret_bind]
+      exact pass_inr_eq_wbisim h
+    · obtain rfl := (Sum.inr.injEq _ _).mp h
+      rename_i h₁ h₂
+      dsimp [sem, Bind.bind]
+      apply WBisim.bind_congr <| pass_inr_eq_wbisim h₁
+      intro k
+      exact pass_inl_eq_wbisim h₂
+    · obtain rfl := (Sum.inr.injEq _ _).mp h
+      rename_i h₁ h₂
+      dsimp [sem, Bind.bind]
+      apply WBisim.bind_congr <| pass_inr_eq_wbisim h₁
+      intro k
+      exact pass_inr_eq_wbisim h₂
+  | .ite c t f => by
+    dsimp [pass, sem, Bind.bind] at h ⊢
+    split at h
+    · rename_i h'
+      apply WBisim.trans <| WBisim.bind_congr_arg <| pass_inl_eq_wbisim h'
+      simp only [ite_not, ret_bind, ↓reduceIte]
+      exact pass_inr_eq_wbisim h
+    · rename_i h'
+      apply WBisim.trans <| WBisim.bind_congr_arg <| pass_inl_eq_wbisim h'
+      simp only [Nat.succ_eq_add_one, Int.ofNat_eq_natCast, Int.natCast_add, Int.cast_ofNat_Int,
+        ite_not, ret_bind]
+      split
+      · omega
+      · exact pass_inr_eq_wbisim h
+    · rename_i h'
+      apply WBisim.trans <| WBisim.bind_congr_arg <| pass_inl_eq_wbisim h'
+      simp only [ite_not, ret_bind, Int.negSucc_ne_zero, ↓reduceIte]
+      exact pass_inr_eq_wbisim h
+    · obtain rfl := (Sum.inr.injEq _ _).mp h
+      rename_i h'
+      apply WBisim.bind_congr <| pass_inr_eq_wbisim h'
+      intro k
+      dsimp
+      split
+      · exact constProp_safe
+      · exact constProp_safe
+  | .while c b => by
+    dsimp [pass, sem, Bind.bind] at h ⊢
+    split at h
+    any_goals contradiction
+    all_goals obtain rfl := (Sum.inr.injEq _ _).mp h
+    all_goals clear h
+    all_goals simp only [ite_not, sem, ne_eq]
+    all_goals apply WBisim.iter_congr_cont
+    all_goals intro k
+    all_goals simp only [Bind.bind, ret_bind, one_ne_zero, ↓reduceIte]
+    all_goals rename_i heq
+    case h_4 =>
+      apply WBisim.bind_congr <| pass_inr_eq_wbisim heq
+      intro c
+      simp only
+      split
+      · rfl
+      · exact WBisim.bind_congr_arg constProp_safe
+    all_goals apply WBisim.trans <| WBisim.bind_congr_arg <| pass_inl_eq_wbisim heq
+    all_goals simp only [Nat.succ_eq_add_one, Int.ofNat_eq_natCast, Int.natCast_add,
+      Int.cast_ofNat_Int, ret_bind, ret_bind, Int.negSucc_ne_zero, ↓reduceIte]
+    any_goals split
+    any_goals omega
+    all_goals exact WBisim.bind_congr_arg constProp_safe
+
+theorem constProp_safe {N} {b : Imp N} : sem b ≈ sem (flat (pass b)) := by
+  cases h : pass b
+  · exact pass_inl_eq_wbisim h
+  · exact pass_inr_eq_wbisim h
+end
+
