sme/Sme/ITree/Interp.lean
@@ -2,13 +2,11 @@ import Sme.ITree.Defs
 import Sme.ITree.Bisim
 import Sme.ITree.Monad
 import Sme.ITree.Combinators
+import Sme.ITree.MonadIter
 
 namespace Sme.ITree
 
 universe u v w
-
-class Iter (M : Type u → Type _) where
-  iter {A B : Type u} : (A → M (A ⊕ B)) → A → M B
 
 instance {E : Type _ → Type _} : Iter (ITree E) where
   iter := ITree.iter
@@ -22,12 +20,8 @@ def interp {E : Type u → Type u} {M : Type (u + 1) → Type _}
     | .vis e k => (.inl ∘ ITree.dest ∘ k ∘ PLift.down) <$> inp _ e
     | .tau x => pure <| .inl x.dest) v.dest
 
-instance {σ : Type u} {M : Type _ → Type _} [Iter M] [Functor M]
-    : Iter (StateT σ M) where
-  iter f a s := Iter.iter (fun ⟨a, s⟩ => (fun
-    | ⟨.inl x, y⟩ => .inl ⟨x, y⟩
-    | ⟨.inr x, y⟩ => .inr ⟨x, y⟩
-    ) <$> f a s) (Prod.mk a s)
+/- br 2  (br 2 (a, b), br 2 (c, d)) ≈ br 4 (a, b, c, d) ≈? br 4 (b, c, d, a)  -/
+/- Strong → Eq -/
 
 end Sme.ITree
 
