sme/Sme/ITree/MonadIter.lean
@@ -1,0 +1,4 @@
+universe u v w
+
+class Iter (M : Type u → Type _) where
+  iter {A B : Type u} : (A → M (A ⊕ B)) → A → M B
